\input{header.tex} \title{Основные понятия}

\begin{document}  

%TODO исправить \sim^\Phi_i
\frame{
\begin{block}{}\textbf{Утверждение}. Пусть $X, Y \in W^\Phi$, тогда
\alert{$ X \not \sim^\Phi_i Y \Rightarrow \; \vdash \underline{X} \to K_i \neg \underline{Y}$}
\end{block}

\resizebox{1.8\textheight}{!}{ 
\begin{fitch}
\fh X \not \sim^\Phi_i Y & $\rhd \; \vdash \underline{X} \to K_i \neg \underline{Y} $ \\
\fa \exists \theta \in \Phi: K_i \theta \in X, \theta \not \in Y \text{ или }
K_i \theta \in Y, \theta \not \in X \\
\fa \fh K_i \theta \in X, \theta \not \in Y  & $\rhd \; \vdash \underline{X} \to K_i \neg \underline{Y} $ \\
\fa \fa \neg \theta \in Y & экономное отрицание? \\
\fa \fa Y \vdash \neg \theta \\
\fa \fa \vdash \underline{Y}  \to \neg \theta \\
\fa \fa \vdash \theta \to \neg \underline{Y}   \\
\fa \fa \vdash K_i \theta \to K_i \neg \underline{Y}   \\
\fa \fa \vdash \underline{X} \to K_i \theta \\
\fa \fa \vdash \underline{X} \to K_i \neg \underline{Y} \\
\fa \fh K_i \theta \in Y, \theta \not \in X & $\rhd \; \vdash \underline{X} \to K_i \neg \underline{Y} $  \\
\fa \fa \neg \theta \in X 
\end{fitch} 
\begin{fitch}
\ftag{13}{\fa \fa \vdash \underline{X} \to \neg \theta}  & \setcounter{fitchcounter}{13}  \\
\fa \fa \vdash \theta \to  \neg \underline{X} \\
\fa \fa \vdash K_i \theta \to  K_i \neg \underline{X} \\
\fa \fa \vdash \underline{Y} \to K_i \theta \\
\fa \fa \vdash \underline{Y} \to K_i \neg \underline{X} \\
\fa \fa \vdash \hat{K}_i \underline{X}  \to \neg \underline{Y} \\
\fa \fa \vdash K_i \hat{K}_i \underline{X}  \to K_i \neg \underline{Y} \\
\fa \fa \vdash \underline{X} \to K_i \hat{K}_i \underline{X} \\
\fa \fa \vdash  \underline{X} \to K_i \neg \underline{Y} \\
\fa \vdash  \underline{X} \to K_i \neg \underline{Y}
\end{fitch}
 }
}

\frame{
\begin{block}{}\textbf{Следствие.} Пусть $X, Y \in W^\Phi$, тогда $\underline{X}, \hat{K}_i \underline{Y} \not \vdash \bot \Rightarrow
X \sim^\Phi_i Y  $	
\end{block}
}

\frame{\frametitle{$\varphi'= K_i \varphi$ ($\Rightarrow$)}
\begin{fitch}
\fh K_i \varphi \in X & $\rhd \; M^\Phi, X \models K_i \varphi \Leftrightarrow \rhd \; \forall Y (X\sim^\Phi_iY \Rightarrow M^\Phi, Y \models \varphi )$ \\ 
\fa \fh \fw{Y} \; X\sim^\Phi_iY & $\rhd \; M^\Phi, Y \models \varphi $ \\
\fa \fa K_i \varphi \in Y & из 1, 2 \\
\fa \fa \varphi \in Y & из 3 т.к. $\varphi \in \Phi$ и $\vdash K_i \varphi \to \varphi$ \\ 
\fa \fa M^\Phi, Y \models \varphi & из 4 по ПИ \\
\fa \forall Y (X\sim^\Phi_iY \Rightarrow M^\Phi, Y \models \varphi) \\
\fa M^\Phi, X \models K_i \varphi 
\end{fitch}
}

\frame{\frametitle{$\varphi'= K_i \varphi$ ($\Leftarrow$)}
Обозначения: $\boxed{K_i X:= \{ K_i  \psi \mid K_i \psi \in X \} }$, $\boxed{\neg K_i X:= \{ \neg K_i \psi \mid \neg K_i \psi \in X \} }$
\resizebox{1.8\textheight}{!}{
\begin{fitch}
\fh	K_i \varphi \not \in X & $\rhd \; M^\Phi, X \not \models K_i \varphi \Leftrightarrow \rhd \; \exists  Y (X\sim^\Phi_iY \wedge M^\Phi, Y \not \models \varphi )$ \\
\fa \neg K_i \varphi \in X \\ 
\fa \vdash \underline{X} \to \neg K_i \varphi \\
\fa \fh y_0 = K_i X \cup  \neg K_i X \cup \{ \neg \varphi \} \vdash \bot & $\rhd \; \metabot$ \\
\fa \fa K_i X, \neg K_i X  \vdash \varphi \\
\fa \fa \vdash ((K_i \psi_1 \wedge \dots \wedge K_i \psi_n) \wedge
(\neg K_i \chi_1 \wedge \dots \wedge \neg K_i \chi_m)) \to  \varphi \\
\fa \fa \vdash K_i ((K_i \psi_1 \wedge \dots \wedge K_i \psi_n) \wedge
(\neg K_i \chi_1 \wedge \dots \wedge \neg K_i \chi_m)) \to  K_i \varphi  \\
\fa \fa \vdash  ((K_i K_i \psi_1 \wedge \dots \wedge K_i K_i \psi_n) \wedge
(K_i \neg K_i \chi_1 \wedge \dots \wedge K_i \neg K_i \chi_m)) \to  K_i \varphi \\
\fa \fa \vdash  ((K_i \psi_1 \wedge \dots \wedge K_i \psi_n) \wedge
(\neg K_i \chi_1 \wedge \dots \wedge \neg K_i \chi_m)) \to  K_i \varphi \\
\fa \fa 
\vdash \underline{X} \to ((K_i \psi_1 \wedge \dots \wedge K_i \psi_n) \wedge
(\neg K_i \chi_1 \wedge \dots \wedge \neg K_i \chi_m)) \\
\fa \fa \vdash \underline{X} \to K_i \varphi \\
\fa \fa \metabot \\
\fa y_0 = K_i X \cup  \neg K_i X \cup \{ \neg \varphi \} \not \vdash \bot 
\end{fitch}
  }
}

\end{document}